day05: Prove confluence of react_step

sol/day05_common.v
@@ -3,6 +3,8 @@ Set Warnings "-extraction-opaque-accessed".
 From Coq Require Import
      Ascii String List Arith
      OrderedTypeEx FMapAVL
+     Sets.Relations_3_facts
+     Relations.Relations
      extraction.ExtrOcamlIntConv.
 Import ListNotations.
 
@@ -52,71 +54,169 @@ Definition react (cs : list int) : list int :=
 
 Section spec.
 
-Context {A : Type}.
-Context (can_react : A -> A -> Prop).
-
-Variant react_step : list A -> list A -> Prop :=
-| RStep (c1 c2 : A) (cs1 cs2 : list A) :
-    can_react c1 c2 ->
-    react_step (cs1 ++ c1 :: c2 :: cs2) (cs1 ++ cs2).
-
-(* Reflexive transitive closure of [react_step]. *)
-Inductive react_steps : list A -> list A -> Prop :=
-| Steps0 (cs : list A) : react_steps cs cs
-| Steps1 (cs cs' cs'' : list A) :
-    react_step  cs  cs'  ->
-    react_steps cs' cs'' ->
-    react_steps cs  cs''
-.
-
-(* [can_react] should be an involutive function. *)
-Hypothesis can_react_symmetric :
-  forall a b, can_react a b -> can_react b a.
-Hypothesis can_react_function :
-  forall a b c, can_react a b -> can_react a c -> b = c.
-
-Lemma can_react_cofunction :
-  forall a b c, can_react a c -> can_react b c -> a = b.
-Proof.
-  intros; eapply can_react_function, can_react_symmetric; eauto.
-Qed.
-
 Ltac gd xs :=
   match xs with
   | (?xs, ?x) => generalize dependent x; gd xs
   | ?x => generalize dependent x
   end.
 
-(* The top and left sides of the square imply the right and bottom
-   ones.
+Section react_generic.
 
-     cs0 > cs1
-      v     v
-     cs2 > cs3
+Context {A : Type}.
 
+Class Reactive : Type :=
+  can_react : A -> A -> Prop.
+Context `{Reactive}.
+
+Variant react_step : list A -> list A -> Prop :=
+| RStep (cs1 : list A) (c1 c2 : A) (cs2 : list A) :
+    can_react c1 c2 ->
+    react_step (cs1 ++ c1 :: c2 :: cs2) (cs1 ++ cs2).
+
+(* Reflexive transitive closure:
+   [react_steps x z] holds when [x] can reach [z] after some
+   number of [react_step]. *)
+Definition react_steps := Rstar _ react_step.
+
+Lemma react_cons_congr1 :
+  forall c cs1 cs2,
+    react_step cs1 cs2 -> react_step (c :: cs1) (c :: cs2).
+Proof.
+  intros ? ? ? [cs1 c1 c2 cs2].
+  apply (RStep (c :: cs1)); auto.
+Qed.
+
+Lemma react_cons_congr :
+  forall c cs1 cs2,
+    react_steps cs1 cs2 ->
+    react_steps (c :: cs1) (c :: cs2).
+Proof.
+  induction 1.
+  - constructor.
+  - econstructor; [|eauto]. apply react_cons_congr1; auto.
+Qed.
+
+Class GoodReactive : Prop := {
+(* [can_react] should be an involutive function. *)
+  can_react_symmetric :
+    forall a b, can_react a b -> can_react b a;
+  can_react_function :
+    forall a b c, can_react a b -> can_react a c -> b = c;
+}.
+
+Context `{GoodReactive}.
+
+Lemma can_react_cofunction :
+  forall a b c, can_react a c -> can_react b c -> a = b.
+Proof.
+  intros; eapply can_react_function; eapply can_react_symmetric; eauto.
+Qed.
+
+(* We prove that [react_step] is [Confluent], i.e., the top and left
+   sides of the following square imply the right and bottom ones.
+
+     cs0 > ... > cs1
+      v           v
+     ...         ...
+      v           v
+     cs2 > ... > cs3
  *)
-Lemma react_step_confluent :
-  forall cs0 cs1 cs2,
-    react_step cs0 cs1 -> react_step cs0 cs2 ->
-    cs1 = cs2 \/ (exists cs3,
-                     react_step cs1 cs3 /\ react_step cs2 cs3).
+
+(* To prove that [react_step] is confluent: it is sufficient to
+   show that it is *locally confluent* and *noetherian*. *)
+
+(* [Locally_confluent]: the top and left sides of the square imply
+   the right and bottom ones.
+
+     x  >  y1
+     v     v*
+     y2 >* z
+ *)
+Lemma Locally_confluent_react_step : Locally_confluent _ react_step.
 Proof.
   intros cs0 cs1 cs2 H01 H02.
   inversion H01; inversion H02; clear H01 H02.
-  gd (cs1, cs2, c1, c2, cs4, c0, c3, cs5, cs6).
+  gd (cs0, cs1, cs2, cs5).
   induction cs3; simpl; intros.
-  - destruct cs5 as [|c5' cs5]; simpl in *.
-    + left; subst. inversion H3; subst; auto.
-    + destruct cs5; simpl in *.
-      * left; subst. inversion H3; subst. f_equal.
-        eapply can_react_function; eauto.
-      * right; subst. inversion H3; subst.
-        exists (cs5 ++ cs6).
-        split.
-        { apply RStep; auto. }
-        { apply (RStep _ _ []); auto. }
-  - admit.
-Abort.
+  - destruct cs5 as [|c5' cs5]; simpl in *; subst.
+    + exists cs1; inversion H5; subst; split; constructor.
+    + destruct cs5; simpl in *; subst.
+      * exists cs1; inversion H5; subst.
+        apply can_react_symmetric in H1.
+        eapply can_react_function in H1; eauto; subst.
+        split; constructor.
+      * exists (cs5 ++ cs6); inversion H5; subst.
+        split; apply Rstar_contains_R.
+        -- apply RStep; auto.
+        -- apply (RStep []); auto.
+  - destruct cs5; simpl in *.
+    + destruct cs3; simpl in *; subst.
+      * exists cs2; inversion H5; subst.
+        eapply can_react_symmetric,
+               (can_react_function _ a c2) in H4; eauto.
+        subst; split; constructor.
+      * exists (cs3 ++ cs4); inversion H5; subst.
+        split; apply Rstar_contains_R.
+        -- apply (RStep []); auto.
+        -- apply RStep; auto.
+    + specialize IHcs3 with (cs5 := cs5).
+      subst; inversion H5; subst; clear H5.
+      edestruct IHcs3 as [cs7 [Hcs7 Hcs7']]; eauto.
+      exists (a :: cs7).
+      split; apply react_cons_congr; auto.
+Qed.
+
+(* [Noetherian]: there is no infinite sequence of steps.
+   In this case, the length decreases by two. *)
+Lemma Noetherian_react_step : Noetherian _ react_step.
+Proof.
+  intros cs.
+  (* Well-founded induction on [length cs]. *)
+  remember (length cs) as n; generalize dependent cs;
+    induction (lt_wf n) as [n Hn IH].
+  constructor; intros cs1 Hcs1.
+  eapply IH; eauto.
+  destruct Hcs1; subst.
+  repeat rewrite app_length.
+  apply Nat.add_lt_mono_l. simpl; auto.
+Qed.
+
+Theorem Confluent_react_step : Confluent _ react_step.
+Proof.
+  apply Newman.
+  - apply Noetherian_react_step.
+  - apply Locally_confluent_react_step.
+Qed.
+
+(* As a corollary, fully reacting a polymer yields a unique result,
+   showing that there is only one possible answer. *)
+
+(* [cs] is inert if it can no longer react. *)
+Definition inert (cs : list A) : Prop :=
+  forall cs', ~ react_step cs cs'.
+
+Definition fully_react (cs cs' : list A) : Prop :=
+  react_steps cs cs' /\ inert cs'.
+
+Corollary react_steps_injective :
+  forall cs cs1 cs2,
+    fully_react cs cs1 ->
+    fully_react cs cs2 ->
+    cs1 = cs2.
+Proof.
+  intros cs cs1 cs2 [Hcs1 Hinert1] [Hcs2 Hinert2].
+  pose proof (Confluent_react_step cs cs1 cs2 Hcs1 Hcs2) as Hconfl.
+  destruct Hconfl as [cs3 [Hcs13 Hcs23]].
+  destruct Hcs13.
+  - destruct Hcs23.
+    + reflexivity.
+    + exfalso; eapply Hinert2; eauto.
+  - exfalso; eapply Hinert1; eauto.
+Qed.
+
+End react_generic.
+
+Global Arguments Reactive : clear implicits.
 
 End spec.
 
@@ -124,11 +224,12 @@ Section example.
 Definition A := 0. Definition a := 1.
 Definition B := 2. Definition b := 3.
 Definition C := 4. Definition c := 5.
-Definition can_react_nat (x y : nat) : Prop := S x = y \/ x = S y.
+Instance Reactive_nat : Reactive nat :=
+  fun (x y : nat) => S x = y \/ x = S y.
 Fixpoint react_list (css : list (list nat)) : Prop :=
   match css with
   | cs :: (cs' :: _) as css =>
-    react_step can_react_nat cs cs' /\
+    react_step cs cs' /\
     react_list css
   | _ => True
   end.
@@ -140,8 +241,8 @@ Example react_ex :
      [C;B;A]].
 Proof.
   repeat constructor.
-  - eapply (RStep _ c C [A]). right;auto.
-  - eapply (RStep _ A a []). left;auto.
-  - eapply (RStep _ c C [_; _; _]). right; auto.
+  - eapply (RStep [A]). right;auto.
+  - eapply (RStep []). left;auto.
+  - eapply (RStep [_; _; _]). right; auto.
 Qed.
 End example.
